Start on program logic

src/MicroSail/Sep/Logic.v
@@ -2,7 +2,7 @@ Require Import Coq.Program.Tactics.
 Require Import FunctionalExtensionality.
 
 (* Adopted from VST: https://github.com/PrincetonUniversity/VST/blob/master/msl/seplog.v *)
-Class NatDed (A: Set) := mkNatDed {
+Class NatDed (A: Type) := mkNatDed {
   andp : A -> A -> A;
   orp : A -> A -> A;
   (* existential quantification *)
@@ -28,13 +28,13 @@ Notation "'∃' x .. y , P " :=
   (exp (fun x => .. (exp (fun y => P%logic)) ..)) (at level 65, x binder, y binder, right associativity) : logic.
 Notation "'∀' x .. y , P " :=
   (allp (fun x => .. (allp (fun y => P%logic)) ..)) (at level 65, x binder, y binder, right associativity) : logic.
-Infix "||" := orp (at level 50, left associativity) : logic.
-Infix "&&" := andp (at level 40, left associativity) : logic.
+Infix "∨" := orp (at level 50, left associativity) : logic.
+Infix "∧" := andp (at level 40, left associativity) : logic.
 Notation "P '-->' Q" := (imp P Q) (at level 55, right associativity) : logic.
 Notation "P '<-->' Q" := (andp (imp P Q) (imp Q P)) (at level 57, no associativity) : logic.
 Notation "'!!' e" := (prop e) (at level 25) : logic.
 
-Class NatDedAxioms (A : Set) := {
+Class NatDedAxioms (A : Type) := {
   isNatDed :> NatDed A;
 
   pred_ext : forall P Q, P ⊢ Q -> Q ⊢ P ->
@@ -44,24 +44,24 @@ Class NatDedAxioms (A : Set) := {
                            P ⊢ R;
 
   andp_right :  forall X P Q, X ⊢ P -> X ⊢ Q ->
-                         X ⊢ P && Q;
+                         X ⊢ P ∧ Q;
   andp_left1 :  forall P Q R, P ⊢ R ->
-                         P && Q ⊢ R;
+                         P ∧ Q ⊢ R;
   andp_left2 :  forall P Q R, Q ⊢ R ->
-                         P && Q ⊢ R;
+                         P ∧ Q ⊢ R;
   orp_left : forall P Q R, P ⊢ R -> Q ⊢ R ->
-                      P || Q ⊢ R;
+                      P ∨ Q ⊢ R;
   orp_right1 : forall P Q R, P ⊢ Q ->
-                        P ⊢ Q || R;
+                        P ⊢ Q ∨ R;
   orp_right2 : forall P Q R, P ⊢ R ->
-                        P ⊢ Q || R;
+                        P ⊢ Q ∨ R;
   exp_right : forall {B : Set} (x : B) (P: A) (Q: B -> A), P ⊢ (Q x) ->
                                                      P ⊢ (exp Q);
   exp_left : forall {B : Set} (P : B -> A) (Q : A),
        (forall x, (P x) ⊢ Q) -> (exp P) ⊢ Q;
   allp_left : forall {B : Set} (P: B -> A) x Q, (P x) ⊢ Q -> (allp P) ⊢ Q;
   allp_right : forall {B : Set} (P: A) (Q: B -> A),  (forall v, P ⊢ (Q v)) -> P ⊢ (allp Q);
-  imp_andp_adjoint : forall P Q R, P && Q ⊢ R <-> P ⊢ (Q --> R);
+  imp_andp_adjoint : forall P Q R, P ∧ Q ⊢ R <-> P ⊢ (Q --> R);
   (* prop_left: forall (P: Prop) Q, (P -> TT ⊢ Q) -> (prop P) ⊢ Q; *)
   (* prop_right: forall (P: Prop) Q, P -> ⊢ Q (prop P); *)
   (* prop_imp_prop_left: forall (P Q: Prop), derives (imp (prop P) (prop Q)) (prop (P -> Q)); *)
@@ -86,7 +86,7 @@ Next Obligation.
 Qed.
 Admit Obligations.
 
-Class SepLog (A : Set) {ND: NatDed A} := mkSepLog {
+Class SepLog (A : Type) {ND: NatDed A} := mkSepLog {
   emp : A;
   sepcon : A -> A -> A;
   wand : A -> A -> A;
@@ -94,19 +94,20 @@ Class SepLog (A : Set) {ND: NatDed A} := mkSepLog {
   ewand : A -> A -> A;
 }.
 
-Notation "P '*' Q" := (sepcon P Q) : logic.
-Notation "P '-*' Q" := (wand P Q) (at level 60, right associativity) : logic.
-Notation "P '-o' Q" := (ewand P Q) (at level 60, right associativity) : logic.
+Notation "P '✱' Q" := (sepcon P Q) (at level 45, left associativity) : logic.
+Notation "P '-✱' Q" := (wand P Q) (at level 60, right associativity) : logic.
+Notation "P '-◯' Q" := (ewand P Q) (* Typeset with -\ci5 *)
+  (at level 60, right associativity) : logic.
 
-Class SepLogAxioms (A : Set) {ND : NatDedAxioms A} := {
+Class SepLogAxioms (A : Type) {ND : NatDedAxioms A} := {
   is_SepLog :> SepLog A;
-  sepcon_assoc: forall (P Q R : A), (P * Q) * R = P * (Q * R);
-  sepcon_comm:  forall (P Q : A), P * Q = Q * P;
-  wand_sepcon_adjoint: forall (P Q R : A), (P * Q ⊢ R) <-> (P ⊢ Q -* R);
-  sepcon_andp_prop: forall (P R : A) (Q : Prop), P * (!!Q && R) = !!Q && (P * R);
-  sepcon_derives: forall P P' Q Q' : A, P ⊢ P' -> Q ⊢ Q' -> P * Q ⊢ P' * Q';
-  ewand_sepcon: forall (P Q R : A),  (P * Q) -o R = P -o (Q * R);
-  ewand_TT_sepcon: forall (P Q R: A), (P * Q) && (R -o TT) ⊢ (P && (R -o TT)) * (Q && (R -o TT));
-  exclude_elsewhere: forall (P Q : A), P * Q ⊢ (P && (Q -o TT)) * Q;
-  ewand_conflict: forall (P Q R : A), P * Q ⊢ FF -> P && (Q -o R) ⊢ FF
+  sepcon_assoc: forall (P Q R : A), (P ✱ Q) ✱ R = P ✱ (Q ✱ R);
+  sepcon_comm:  forall (P Q : A), P ✱ Q = Q ✱ P;
+  wand_sepcon_adjoint: forall (P Q R : A), (P ✱ Q ⊢ R) <-> (P ⊢ Q -✱ R);
+  sepcon_andp_prop: forall (P R : A) (Q : Prop), P ✱ (!!Q ∧ R) = !!Q ∧ (P ✱ R);
+  sepcon_derives: forall P P' Q Q' : A, P ⊢ P' -> Q ⊢ Q' -> P ✱ Q ⊢ P' ✱ Q';
+  ewand_sepcon: forall (P Q R : A),  (P ✱ Q) -◯ R = P -◯ (Q ✱ R);
+  ewand_TT_sepcon: forall (P Q R: A), (P ✱ Q) ∧ (R -◯ TT) ⊢ (P ∧ (R -◯ TT)) ✱ (Q ∧ (R -◯ TT));
+  exclude_elsewhere: forall (P Q : A), P ✱ Q ⊢ (P ∧ (Q -◯ TT)) ✱ Q;
+  ewand_conflict: forall (P Q R : A), P ✱ Q ⊢ FF -> P ∧ (Q -◯ R) ⊢ FF
 }.
