src/MicroSail/Sep/Hoare.v
@@ -1,0 +1,44 @@
+Require Import Coq.Program.Tactics.
+Require Import FunctionalExtensionality.
+
+Require Import MicroSail.Syntax.
+Require Import MicroSail.Sep.Logic.
+
+Module ProgramLogic
+
+  (Import typekit : TypeKit)
+  (Import termkit : TermKit typekit)
+  (Import progKit : ProgramKit typekit termkit).
+
+  Import CtxNotations.
+  Import EnvNotations.
+
+  Open Scope logic.
+  Definition ctxprop := Ctx (𝑿 * Ty) -> Prop.
+
+  Definition ptstoctx {Γ : Ctx (𝑿 * Ty)} {A : Set} (x : 𝑿) (v : A) : ctxprop :=
+    fun _ => True.
+
+  Program Instance ctxpop_NatDed : NatDed ctxprop.
+  Admit Obligations.
+
+
+
+  Reserved Notation "⦃ P ⦄ s ⦃ Q ⦄" (at level 75, no associativity).
+  Inductive Triple
+            (* {A : Set} {ND : NatDedAxioms A} {SL : SepLogAxioms A} *)
+            {Γ : Ctx (𝑿 * Ty)} :
+            forall {σ : Ty}
+            (pre : ctxprop) (s : Stm Γ σ) (post : ctxprop), Prop :=
+    | rule_stm_lit (σ : Ty) (l : Lit σ) : forall (P : ctxprop), ⦃ P ⦄ stm_lit σ l ⦃ P ⦄
+    | rule_stm_exp (σ : Ty) (e : Exp Γ σ) : forall (P : ctxprop), ⦃ P ⦄ stm_exp e ⦃ P ⦄
+    | rule_stm_let (x : 𝑿) (τ : Ty) (s : Stm Γ τ) {σ : Ty}
+                   (k : Stm (ctx_snoc Γ (x , τ)) σ) :
+        forall (P : ctxprop), ⦃ P ⦄ let: x := s in k ⦃ P ⦄
+    where "⦃ P ⦄ s ⦃ Q ⦄" := (Triple P s Q).
+
+(x : 𝑿) (τ : Ty) (s : Stm Γ τ) {σ : Ty} (k : Stm (ctx_snoc Γ (x , τ)) σ) : Stm Γ σ
+      | rule_stm_exp
+        TT (stm_exp ) FF.
+      (γ : RegStore) (μ : Memory) (δ : LocalStore Γ) (σ : Ty) (e : Exp Γ σ) :
+      ⟨ γ , μ , δ , (stm_exp e) ⟩ ---> ⟨ γ , μ , δ , stm_lit σ (eval e δ) ⟩
